uniana/cfg/HeadRewireDeqMh.v
@@ -1,0 +1,86 @@
+Require Export HeadRewire.
+
+Section cfg.
+  Context `(C : redCFG).
+
+  Infix "-h>" := (head_rewired_edge) (at level 70).
+
+
+  Definition loop_contains_strict h p
+    := loop_contains h p /\ h <> p.
+
+  Definition deq_loop_mh q p
+    := forall h, h <> p -> loop_contains h p -> loop_contains h q.
+
+  Definition eq_loop_mh q p
+    := deq_loop_mh q p /\ deq_loop_mh p q.
+
+  Lemma eq_loop_mh_sym : Symmetric eq_loop_mh.
+  Proof.
+    firstorder.
+  Qed.
+
+  Instance deq_loop_mh_refl : Reflexive deq_loop_mh.
+  Proof.
+    unfold Reflexive. intros x h Hloop Hneq.
+    auto.
+  Qed.
+
+  Lemma deq_loop_deq_loop_mh p q
+        (Hdeq : deq_loop p q)
+    : deq_loop_mh p q.
+  Proof.
+    intros h Hloop Hneq.
+    eauto.
+  Qed.
+
+  Lemma deq_loop_mh_deq_loop p q
+        (Hnh : ~ loop_head q)
+        (Hdeq : deq_loop_mh p q)
+    : deq_loop p q.
+  Proof.
+    intros h Hloop.
+    eapply Hdeq.
+    - contradict Hnh. subst h. eapply loop_contains_loop_head;eauto.
+    - assumption.
+  Qed.
+
+  Lemma head_rewired_deq_loop_mh p q
+        (Hedge : p -h> q)
+    : deq_loop_mh p q.
+  Proof.
+    destruct Hedge.
+    - destructH. destruct (edge_Edge H0);intros h Hloop Hneq.
+      + eapply basic_edge_eq_loop in b.
+        rewrite b. auto.
+      + eapply back_edge_eq_loop in b. rewrite b. assumption.
+      + eapply deq_loop_entry_or in e;eauto.
+        destruct e;[assumption|contradiction].
+      + destruct e. eapply deq_loop_exited;eauto.
+    - destruct H. intros h Hloop Hneq.
+      eapply deq_loop_exited';eauto.
+  Qed.
+
+  Lemma hpath_deq_loop_mh p q π
+        (Hpath : HPath p q π)
+    : deq_loop_mh p q.
+  Proof.
+    induction Hpath.
+    - reflexivity.
+    - eapply head_rewired_deq_loop_mh in H as Hmh.
+      intros h Hneq Hloop.
+      eapply IHHpath;eauto.
+      contradict Hloop.
+      subst h. eapply head_rewired_not_contains;eauto.
+  Qed.
+
+  Lemma hpath_deq_loop_mh_elem p q π x
+        (Hpath : HPath p q π)
+        (Hin : x ∈ π)
+    : deq_loop_mh x q.
+  Proof.
+    eapply path_from_elem in Hpath;eauto.
+    destructH.
+    eapply hpath_deq_loop_mh;eauto.
+  Qed.
+End cfg.
